flake.nix
@@ -1,0 +1,21 @@
+{
+  description = "A separation logic for cryptographic protocols";
+
+  inputs = {
+    nixpkgs.url = "github:nixos/nixpkgs";
+  };
+
+  outputs = { self, nixpkgs }:
+
+    let pkgs = nixpkgs.legacyPackages.x86_64-linux; in {
+          devShell.x86_64-linux =
+            pkgs.mkShell {
+              buildInputs = with pkgs; [
+                coq
+                coqPackages.mathcomp.ssreflect
+                coqPackages.iris
+                coqPackages.deriving
+              ];
+            };
+        };
+}
